Used Rcompare to reduce inbetween's disjunction to only Exact/Inexact. Simplified proofs.

src/Calc/Fcalc_bracket.v
@@ -2,70 +2,12 @@ Require Import Fcore.
 
 Section Fcalc_bracket.
 
-Lemma Rhalf_lt_compat :
-  forall x y, (x < y)%R -> (x / 2 < y / 2)%R.
-Proof.
-intros x y.
-apply Rmult_lt_compat_r.
-apply Rinv_0_lt_compat.
-now apply (Z2R_lt 0 2).
-Qed.
-
-Lemma Rhalf_le_compat :
-  forall x y, (x <= y)%R -> (x / 2 <= y / 2)%R.
-Proof.
-intros x y.
-apply Rmult_le_compat_r.
-apply Rlt_le.
-apply Rinv_0_lt_compat.
-now apply (Z2R_lt 0 2).
-Qed.
-
-Lemma Rhalf_lt_reg :
-  forall x y, (x / 2 < y / 2)%R -> (x < y)%R.
-Proof.
-intros x y.
-apply Rmult_lt_reg_r.
-apply Rinv_0_lt_compat.
-now apply (Z2R_lt 0 2).
-Qed.
-
-Lemma Rhalf_le_reg :
-  forall x y, (x / 2 <= y / 2)%R -> (x <= y)%R.
-Proof.
-intros x y.
-apply Rmult_le_reg_r.
-apply Rinv_0_lt_compat.
-now apply (Z2R_lt 0 2).
-Qed.
-
 Variable d u : R.
+Hypothesis Hdu : (d < u)%R.
 
 Lemma ordered_middle :
-  (d <= u)%R -> (d <= (d + u)/2 <= u)%R.
+  (d < (d + u)/2 < u)%R.
 Proof.
-intros Hdu.
-split.
-apply Rmult_le_reg_r with 2%R.
-now apply (Z2R_lt 0 2).
-unfold Rdiv.
-rewrite Rmult_assoc, Rinv_l, Rmult_1_r.
-rewrite Rmult_plus_distr_l, Rmult_1_r.
-now apply Rplus_le_compat_l.
-now apply (Z2R_neq 2 0).
-apply Rmult_le_reg_r with 2%R.
-now apply (Z2R_lt 0 2).
-unfold Rdiv.
-rewrite Rmult_assoc, Rinv_l, Rmult_1_r.
-rewrite Rmult_plus_distr_l, Rmult_1_r.
-now apply Rplus_le_compat_r.
-now apply (Z2R_neq 2 0).
-Qed.
-
-Lemma ordered_middle_strict :
-  (d < u)%R -> (d < (d + u)/2 < u)%R.
-Proof.
-intros Hdu.
 split.
 apply Rmult_lt_reg_r with 2%R.
 now apply (Z2R_lt 0 2).
@@ -83,206 +25,104 @@ now apply Rplus_lt_compat_r.
 now apply (Z2R_neq 2 0).
 Qed.
 
-Lemma ordered_low_imp_ordered :
-  (d < (d + u)/2)%R -> (d < u)%R.
-Proof.
-intros Hdu.
-apply Rhalf_lt_reg.
-apply Rplus_lt_reg_r with (d / 2)%R.
-unfold Rdiv.
-rewrite <- 2!Rmult_plus_distr_r.
-pattern d at 1 2 ; rewrite <- Rmult_1_r.
-rewrite <- Rmult_plus_distr_l.
-rewrite Rmult_assoc, Rinv_r.
-now rewrite Rmult_1_r.
-now apply (Z2R_neq 2 0).
-Qed.
-
-Lemma ordered_high_imp_ordered :
-  ((d + u)/2 < u)%R -> (d < u)%R.
-Proof.
-intros Hdu.
-apply Rhalf_lt_reg.
-apply Rplus_lt_reg_r with (u / 2)%R.
-unfold Rdiv.
-rewrite <- 2!Rmult_plus_distr_r.
-pattern u at 2 3 ; rewrite <- Rmult_1_r.
-rewrite <- Rmult_plus_distr_l.
-rewrite Rmult_assoc, Rinv_r.
-now rewrite Rplus_comm, Rmult_1_r.
-now apply (Z2R_neq 2 0).
-Qed.
-
-Inductive location := loc_Eq | loc_Lo | loc_Mi | loc_Hi.
+Inductive location := loc_Exact | loc_Inexact : comparison -> location.
 
 Variable x : R.
 
 Inductive inbetween : location -> Prop :=
-  | inbetween_Eq : x = d -> inbetween loc_Eq
-  | inbetween_Lo : (d < x)%R -> (x < (d + u)/2)%R -> inbetween loc_Lo
-  | inbetween_Mi : x = ((d + u)/2)%R -> inbetween loc_Mi
-  | inbetween_Hi : ((d + u)/2 < x)%R -> (x < u)%R -> inbetween loc_Hi.
+  | inbetween_Exact : x = d -> inbetween loc_Exact
+  | inbetween_Inexact l : (d < x < u)%R -> Rcompare x ((d + u) / 2)%R = l -> inbetween (loc_Inexact l).
 
 Section Fcalc_bracket_any.
 
 Variable l : location.
 
 Theorem inbetween_not_Hi :
-  (d <= u)%R ->
   inbetween l ->
-  l <> loc_Hi ->
+  l <> loc_Inexact Gt ->
   (d <= x <= (d + u)/2)%R.
 Proof.
-intros Hdu [Hx|Hx1 Hx2|Hx|Hx1 Hx2] H ; try (now elim H) ; clear H.
+intros [Hx|[] Hx Hl] H ; try (now elim H) ; clear l H.
 rewrite Hx.
 split.
 apply Rle_refl.
-now eapply ordered_middle.
-split ; now apply Rlt_le.
-rewrite Hx.
+apply Rlt_le.
+apply ordered_middle.
+rewrite Rcompare_Eq_inv with (1 := Hl).
 split.
-now eapply ordered_middle.
+apply Rlt_le.
+apply ordered_middle.
 apply Rle_refl.
+split ; apply Rlt_le.
+apply Hx.
+now apply Rcompare_Lt_inv.
 Qed.
 
 Theorem inbetween_Mi_Hi :
-  (d <= u)%R ->
   inbetween l ->
-  l = loc_Mi \/ l = loc_Hi ->
+  l = loc_Inexact Eq \/ l = loc_Inexact Gt ->
   ((d + u)/2 <= x <= u)%R.
 Proof.
-intros Hdu [Hx|Hx1 Hx2|Hx|Hx1 Hx2] H ; try (now elim H) ; clear H.
-rewrite Hx.
+intros [Hx|[] Hx Hl] H ; try (now elim H) ; clear l H.
+rewrite Rcompare_Eq_inv with (1 := Hl).
 split.
 apply Rle_refl.
-now eapply ordered_middle.
-split ; now apply Rlt_le.
+apply Rlt_le.
+apply ordered_middle.
+split ; apply Rlt_le.
+now apply Rcompare_Gt_inv.
+apply Hx.
 Qed.
 
 Theorem inbetween_bounds :
-  (d <= u)%R ->
   inbetween l ->
-  (d <= x <= u)%R.
+  (d <= x < u)%R.
 Proof.
-intros Hdu [Hx|Hx1 Hx2|Hx|Hx1 Hx2] ; clear l.
+intros [Hx|l' Hx Hl] ; clear l.
 rewrite Hx.
 split.
 apply Rle_refl.
 exact Hdu.
-split.
-now apply Rlt_le.
-apply Rlt_le.
-apply Rlt_le_trans with (1 := Hx2).
-now eapply ordered_middle.
-rewrite Hx.
-now apply ordered_middle.
-split. 2: now apply Rlt_le.
-apply Rlt_le.
-apply Rle_lt_trans with (2 := Hx1).
-now eapply ordered_middle.
+now split ; try apply Rlt_le.
 Qed.
 
-Theorem inbetween_bounds_strict :
-  (d < u)%R ->
+Theorem inbetween_bounds_not_Eq :
   inbetween l ->
-  (d <= x < u)%R.
-Proof.
-intros Hdu Hl.
-split.
-eapply inbetween_bounds.
-now apply Rlt_le.
-exact Hl.
-destruct Hl as [Hx|Hx1 Hx2|Hx|Hx1 Hx2].
-now rewrite Hx.
-apply Rlt_le_trans with (1 := Hx2).
-refine (proj2 (ordered_middle _)).
-now apply Rlt_le.
-rewrite Hx.
-exact (proj2 (ordered_middle_strict Hdu)).
-exact Hx2.
-Qed.
-
-Theorem inbetween_bounds_strict_not_Eq :
-  (d < u)%R ->
-  inbetween l ->
-  l <> loc_Eq ->
+  l <> loc_Exact ->
   (d < x < u)%R.
 Proof.
-intros Hdu Hl.
-split.
-2: exact (proj2 (inbetween_bounds_strict Hdu Hl)).
-destruct Hl as [Hx|Hx1 Hx2|Hx|Hx1 Hx2] ; try (now elim H) ; clear H.
-exact Hx1.
-rewrite Hx.
-exact (proj1 (ordered_middle_strict Hdu)).
-apply Rle_lt_trans with (2 := Hx1).
-refine (proj1 (ordered_middle _)).
-now apply Rlt_le.
+intros [Hx|l' Hx Hl] H.
+now elim H.
+exact Hx.
 Qed.
 
 End Fcalc_bracket_any.
 
-Theorem inbetween_distance_Lo :
-  inbetween loc_Lo ->
-  (Rabs (d - x) < Rabs (u - x))%R.
+Theorem inbetween_distance_inexact :
+  forall l,
+  inbetween (loc_Inexact l) ->
+  Rcompare (x - d) (u - x) = l.
 Proof.
-intros Hl.
-inversion Hl.
-rewrite Rabs_left. 2: now apply Rlt_minus.
+intros l Hl.
+inversion_clear Hl as [|l' Hl' Hx].
+now rewrite Rcompare_middle.
+Qed.
+
+Theorem inbetween_distance_inexact_abs :
+  forall l,
+  inbetween (loc_Inexact l) ->
+  Rcompare (Rabs (d - x)) (Rabs (u - x)) = l.
+Proof.
+intros l Hl.
+rewrite Rabs_left1.
 rewrite Rabs_pos_eq.
 rewrite Ropp_minus_distr.
-apply Rplus_lt_reg_r with (x + d)%R.
-ring_simplify.
-apply Rhalf_lt_reg.
-unfold Rdiv at 1.
-rewrite Rmult_comm, <- Rmult_assoc, Rinv_l, Rmult_1_l.
-exact H0.
-now apply (Z2R_neq 2 0).
+now apply inbetween_distance_inexact.
 apply Rle_0_minus.
 apply Rlt_le.
-apply Rlt_trans with (1 := H0).
-apply ordered_middle_strict.
-apply ordered_low_imp_ordered.
-now apply Rlt_trans with x.
-Qed.
-
-Theorem inbetween_distance_Mi :
-  inbetween loc_Mi ->
-  (x - d = u - x)%R.
-Proof.
-intros Hl.
-inversion Hl.
-apply Rplus_eq_reg_l with (x + d)%R.
-ring_simplify.
-apply Rmult_eq_reg_r with (/2)%R.
-rewrite Rmult_comm, <- Rmult_assoc, Rinv_l, Rmult_1_l.
-exact H.
-now apply (Z2R_neq 2 0).
-apply Rinv_neq_0_compat.
-now apply (Z2R_neq 2 0).
-Qed.
-
-Theorem inbetween_distance_Hi :
-  inbetween loc_Hi ->
-  (Rabs (u - x) < Rabs (d - x))%R.
-Proof.
-intros Hl.
-inversion Hl.
-rewrite Rabs_pos_eq. 2: apply Rle_0_minus ; now apply Rlt_le.
-rewrite Rabs_left.
-rewrite Ropp_minus_distr.
-apply Rplus_lt_reg_r with (x + d)%R.
-ring_simplify.
-apply Rhalf_lt_reg.
-unfold Rdiv at 2.
-rewrite Rmult_comm, <- Rmult_assoc, Rinv_l, Rmult_1_l.
-exact H.
-now apply (Z2R_neq 2 0).
-apply Rlt_minus.
-apply Rlt_trans with (2 := H).
-apply ordered_middle_strict.
-apply ordered_high_imp_ordered.
-now apply Rlt_trans with x.
+apply (inbetween_bounds _ Hl).
+apply Rle_minus.
+apply (inbetween_bounds _ Hl).
 Qed.
 
 End Fcalc_bracket.
@@ -311,129 +151,124 @@ apply Z2R_lt.
 apply Zlt_succ.
 Qed.
 
+Lemma mid_step :
+  forall k,
+  ((start + (start + Z2R k * step)) / 2 = start + (Z2R k / 2 * step))%R.
+Proof.
+intros k.
+field.
+Qed.
+
 Hypothesis (Hnb_steps : (1 < nb_steps)%Z).
 
-Theorem inbetween_step_Lo :
-  forall x k l,
+Lemma inbetween_step_not_Eq :
+  forall x k l l',
   inbetween (start + Z2R k * step) (start + Z2R (k + 1) * step) x l ->
-  (0 < k)%Z -> (2 * k + 1 < nb_steps)%Z ->
-  inbetween start (start + Z2R nb_steps * step) x loc_Lo.
+  (0 < k < nb_steps)%Z ->
+  Rcompare x (start + (Z2R nb_steps / 2 * step))%R = l' ->
+  inbetween start (start + Z2R nb_steps * step) x (loc_Inexact l').
 Proof.
-intros x k l Hx Hk1 Hk2.
+intros x k l l' Hx Hk Hl'.
 constructor.
 (* . *)
-apply Rlt_le_trans with (start + Z2R k * step)%R.
+assert (Hx' := inbetween_bounds _ _ (ordered_steps _) _ _ Hx).
+split.
+apply Rlt_le_trans with (2 := proj1 Hx').
 rewrite <- (Rplus_0_r start) at 1.
 apply Rplus_lt_compat_l.
 apply Rmult_lt_0_compat.
 now apply (Z2R_lt 0).
 exact Hstep.
-refine (proj1 (inbetween_bounds _ _ _ _ _ Hx)).
-apply Rlt_le.
-apply ordered_steps.
-(* . *)
-apply Rlt_le_trans with (start + Z2R (k + 1) * step)%R.
-exact (proj2 (inbetween_bounds_strict _ _ _ _ (ordered_steps _) Hx)).
-rewrite <- Rplus_assoc.
-unfold Rdiv.
-rewrite Rmult_plus_distr_r.
-fold ((start + start)/2)%R.
-rewrite double_div2.
+apply Rlt_le_trans with (1 := proj2 Hx').
 apply Rplus_le_compat_l.
-replace (Z2R nb_steps * step * / 2)%R with (Z2R nb_steps * /2 * step)%R by ring.
 apply Rmult_le_compat_r.
 now apply Rlt_le.
-apply Rmult_le_reg_r with 2%R.
-now apply (Z2R_lt 0 2).
-rewrite Rmult_assoc, Rinv_l, Rmult_1_r.
+apply Z2R_le.
+omega.
+(* . *)
+now rewrite mid_step.
+Qed.
+
+Theorem inbetween_step_Lo :
+  forall x k l,
+  inbetween (start + Z2R k * step) (start + Z2R (k + 1) * step) x l ->
+  (0 < k)%Z -> (2 * k + 1 < nb_steps)%Z ->
+  inbetween start (start + Z2R nb_steps * step) x (loc_Inexact Lt).
+Proof.
+intros x k l Hx Hk1 Hk2.
+apply inbetween_step_not_Eq with (1 := Hx).
+omega.
+apply Rcompare_Lt.
+assert (Hx' := inbetween_bounds _ _ (ordered_steps _) _ _ Hx).
+apply Rlt_le_trans with (1 := proj2 Hx').
+apply Rcompare_not_Lt_inv.
+rewrite Rcompare_plus_l, Rcompare_mult_r, Rcompare_half_l.
+apply Rcompare_not_Lt.
 change 2%R with (Z2R 2).
 rewrite <- mult_Z2R.
 apply Z2R_le.
 omega.
-now apply (Z2R_neq 2 0).
+exact Hstep.
 Qed.
 
 Theorem inbetween_step_Hi :
   forall x k l,
   inbetween (start + Z2R k * step) (start + Z2R (k + 1) * step) x l ->
   (nb_steps < 2 * k)%Z -> (k < nb_steps)%Z ->
-  inbetween start (start + Z2R nb_steps * step) x loc_Hi.
+  inbetween start (start + Z2R nb_steps * step) x (loc_Inexact Gt).
 Proof.
 intros x k l Hx Hk1 Hk2.
-constructor.
-(* . *)
-apply Rlt_le_trans with (start + Z2R k * step)%R.
-rewrite <- Rplus_assoc.
-unfold Rdiv.
-rewrite Rmult_plus_distr_r.
-fold ((start + start)/2)%R.
-rewrite double_div2.
-apply Rplus_lt_compat_l.
-replace (Z2R nb_steps * step * / 2)%R with (Z2R nb_steps * /2 * step)%R by ring.
-apply Rmult_lt_compat_r.
-exact Hstep.
-apply Rmult_lt_reg_r with 2%R.
-now apply (Z2R_lt 0 2).
-rewrite Rmult_assoc, Rinv_l, Rmult_1_r.
+apply inbetween_step_not_Eq with (1 := Hx).
+omega.
+apply Rcompare_Gt.
+assert (Hx' := inbetween_bounds _ _ (ordered_steps _) _ _ Hx).
+apply Rlt_le_trans with (2 := proj1 Hx').
+apply Rcompare_Lt_inv.
+rewrite Rcompare_plus_l, Rcompare_mult_r, Rcompare_half_l.
+apply Rcompare_Lt.
 change 2%R with (Z2R 2).
 rewrite <- mult_Z2R.
 apply Z2R_lt.
-now rewrite Zmult_comm.
-now apply (Z2R_neq 2 0).
-refine (proj1 (inbetween_bounds _ _ _ _ _ Hx)).
-apply Rlt_le.
-apply ordered_steps.
-(* . *)
-apply Rlt_le_trans with (start + Z2R (k + 1) * step)%R.
-exact (proj2 (inbetween_bounds_strict _ _ _ _ (ordered_steps _) Hx)).
-apply Rplus_le_compat_l.
-apply Rmult_le_compat_r.
-now apply Rlt_le.
-apply Z2R_le.
-now apply Zlt_le_succ.
+omega.
+exact Hstep.
 Qed.
 
-Theorem inbetween_step_Lo_Eq :
+Theorem inbetween_step_Lo_not_Eq :
   forall x l,
   inbetween start (start + step) x l ->
-  l <> loc_Eq ->
-  inbetween start (start + Z2R nb_steps * step) x loc_Lo.
+  l <> loc_Exact ->
+  inbetween start (start + Z2R nb_steps * step) x (loc_Inexact Lt).
 Proof.
 intros x l Hx Hl.
+assert (Hx' := inbetween_bounds_not_Eq _ _ _ _ Hx Hl).
 constructor.
 (* . *)
-refine (proj1 (inbetween_bounds_strict_not_Eq _ _ _ _ _ Hx Hl)).
-rewrite <- (Rplus_0_r start) at 1.
-now apply Rplus_lt_compat_l.
-(* . *)
-apply Rlt_le_trans with (start + step)%R.
-refine (proj2 (inbetween_bounds_strict _ _ _ _ _ Hx)).
-rewrite <- (Rplus_0_r start) at 1.
-now apply Rplus_lt_compat_l.
-rewrite <- Rplus_assoc.
-unfold Rdiv.
-rewrite Rmult_plus_distr_r.
-fold ((start + start)/2)%R.
-rewrite double_div2.
-apply Rplus_le_compat_l.
-replace (Z2R nb_steps * step * / 2)%R with (Z2R nb_steps * /2 * step)%R by ring.
+split.
+apply Hx'.
+apply Rlt_trans with (1 := proj2 Hx').
+apply Rplus_lt_compat_l.
 rewrite <- (Rmult_1_l step) at 1.
-apply Rmult_le_compat_r.
-now apply Rlt_le.
-apply Rmult_le_reg_r with 2%R.
-now apply (Z2R_lt 0 2).
-rewrite Rmult_assoc, Rinv_l, Rmult_1_r.
-change 2%R with (Z2R 2).
-rewrite <- (mult_Z2R 1).
-apply Z2R_le.
-exact (Zlt_le_succ _ _ Hnb_steps).
-now apply (Z2R_neq 2 0).
+apply Rmult_lt_compat_r.
+exact Hstep.
+now apply (Z2R_lt 1).
+(* . *)
+apply Rcompare_Lt.
+apply Rlt_le_trans with (1 := proj2 Hx').
+rewrite mid_step.
+apply Rcompare_not_Lt_inv.
+rewrite <- (Rmult_1_l step) at 2.
+rewrite Rcompare_plus_l, Rcompare_mult_r, Rcompare_half_l.
+rewrite Rmult_1_r.
+apply Rcompare_not_Lt.
+apply (Z2R_le 2).
+now apply (Zlt_le_succ 1).
+exact Hstep.
 Qed.
 
 Lemma middle_odd :
   forall k,
   (2 * k + 1 = nb_steps)%Z ->
-  (((start + Z2R k * step) + (start + Z2R (k + 1) * step))/2 = start + Z2R nb_steps * step * /2)%R.
+  (((start + Z2R k * step) + (start + Z2R (k + 1) * step))/2 = start + Z2R nb_steps /2 * step)%R.
 Proof.
 intros k Hk.
 rewrite <- Hk.
@@ -441,158 +276,89 @@ rewrite 2!plus_Z2R, mult_Z2R.
 simpl. field.
 Qed.
 
-Theorem inbetween_step_Lo_Mi_odd :
+Theorem inbetween_step_any_Mi_odd :
   forall x k l,
-  inbetween (start + Z2R k * step) (start + Z2R (k + 1) * step) x l ->
-  l = loc_Eq \/ l = loc_Lo ->
+  inbetween (start + Z2R k * step) (start + Z2R (k + 1) * step) x (loc_Inexact l) ->
   (2 * k + 1 = nb_steps)%Z ->
-  inbetween start (start + Z2R nb_steps * step) x loc_Lo.
+  inbetween start (start + Z2R nb_steps * step) x (loc_Inexact l).
 Proof.
-intros x k l Hx Hl Hk.
-constructor.
-(* . *)
-apply Rlt_le_trans with (start + Z2R k * step)%R.
-rewrite <- (Rplus_0_r start) at 1.
-apply Rplus_lt_compat_l.
-apply Rmult_lt_0_compat with (2 := Hstep).
-apply (Z2R_lt 0).
+intros x k l Hx Hk.
+apply inbetween_step_not_Eq with (1 := Hx).
 omega.
-refine (proj1 (inbetween_bounds _ _ _ _ _ Hx)).
-apply Rlt_le.
-apply ordered_steps.
-(* . *)
-rewrite <- Rplus_assoc.
-unfold Rdiv.
-rewrite Rmult_plus_distr_r.
-fold ((start + start)/2)%R.
-rewrite double_div2.
-destruct Hx as [Hx|Hx1 Hx2|Hx|Hx1 Hx2] ; try (now elim Hl) ; clear Hl.
-(* .. *)
-rewrite Hx.
-apply Rplus_lt_compat_l.
-apply Rmult_lt_reg_r with 2%R.
-now apply (Z2R_lt 0 2).
-rewrite (Rmult_assoc (Z2R nb_steps * step)), Rinv_l, Rmult_1_r.
-replace (Z2R k * step * 2)%R with (Z2R k * 2 * step)%R by ring.
-apply Rmult_lt_compat_r with (1 := Hstep).
+inversion_clear Hx as [|l' _ Hl].
+now rewrite (middle_odd _ Hk) in Hl.
+Qed.
+
+Theorem inbetween_step_Lo_Mi_Eq_odd :
+  forall x k,
+  inbetween (start + Z2R k * step) (start + Z2R (k + 1) * step) x loc_Exact ->
+  (2 * k + 1 = nb_steps)%Z ->
+  inbetween start (start + Z2R nb_steps * step) x (loc_Inexact Lt).
+Proof.
+intros x k Hx Hk.
+apply inbetween_step_not_Eq with (1 := Hx).
+omega.
+inversion_clear Hx as [Hl|].
+rewrite Hl.
+rewrite Rcompare_plus_l, Rcompare_mult_r, Rcompare_half_r.
+apply Rcompare_Lt.
 change 2%R with (Z2R 2).
 rewrite <- mult_Z2R.
 apply Z2R_lt.
-omega.
-now apply (Z2R_neq 2 0).
-(* .. *)
-now rewrite <- middle_odd with (1 := Hk).
-Qed.
-
-Theorem inbetween_step_Hi_Mi_odd :
-  forall x k,
-  inbetween (start + Z2R k * step) (start + Z2R (k + 1) * step) x loc_Hi ->
-  (2 * k + 1 = nb_steps)%Z ->
-  inbetween start (start + Z2R nb_steps * step) x loc_Hi.
-Proof.
-intros x k Hx Hk.
-constructor.
-(* . *)
-rewrite <- Rplus_assoc.
-unfold Rdiv.
-rewrite Rmult_plus_distr_r.
-fold ((start + start)/2)%R.
-rewrite double_div2.
-inversion_clear Hx.
-now rewrite <- middle_odd with (1 := Hk).
-(* . *)
-apply Rlt_le_trans with (start + Z2R (k + 1) * step)%R.
-exact (proj2 (inbetween_bounds_strict _ _ _ _ (ordered_steps _) Hx)).
-apply Rplus_le_compat_l.
-apply Rmult_le_compat_r.
-now apply Rlt_le.
-apply Z2R_le.
-omega.
+rewrite <- Hk.
+apply Zlt_succ.
+exact Hstep.
 Qed.
 
 Theorem inbetween_step_Hi_Mi_even :
   forall x k l,
   inbetween (start + Z2R k * step) (start + Z2R (k + 1) * step) x l ->
-  l <> loc_Eq ->
+  l <> loc_Exact ->
   (2 * k = nb_steps)%Z ->
-  inbetween start (start + Z2R nb_steps * step) x loc_Hi.
+  inbetween start (start + Z2R nb_steps * step) x (loc_Inexact Gt).
 Proof.
 intros x k l Hx Hl Hk.
-constructor.
-(* . *)
-rewrite <- Rplus_assoc.
-unfold Rdiv.
-rewrite Rmult_plus_distr_r.
-fold ((start + start)/2)%R.
-rewrite double_div2.
-replace (Z2R nb_steps * step * / 2)%R with (Z2R k * step)%R.
-exact (proj1 (inbetween_bounds_strict_not_Eq _ _ _ _ (ordered_steps _) Hx Hl)).
-rewrite <- Hk, mult_Z2R.
-simpl (Z2R 2).
-replace (2 * Z2R k * step * / 2)%R with (Z2R k * step * (2 * /2))%R by ring.
-rewrite Rinv_r, Rmult_1_r.
-apply refl_equal.
-now apply (Z2R_neq 2 0).
-(* . *)
-apply Rlt_le_trans with (start + Z2R (k + 1) * step)%R.
-exact (proj2 (inbetween_bounds_strict _ _ _ _ (ordered_steps _) Hx)).
-apply Rplus_le_compat_l.
-apply Rmult_le_compat_r.
-now apply Rlt_le.
-apply Z2R_le.
+apply inbetween_step_not_Eq with (1 := Hx).
 omega.
+apply Rcompare_Gt.
+assert (Hx' := inbetween_bounds_not_Eq _ _ _ _ Hx Hl).
+apply Rle_lt_trans with (2 := proj1 Hx').
+apply Rcompare_not_Lt_inv.
+rewrite Rcompare_plus_l, Rcompare_mult_r, Rcompare_half_r.
+change 2%R with (Z2R 2).
+rewrite <- mult_Z2R.
+apply Rcompare_not_Lt.
+apply Z2R_le.
+rewrite Hk.
+apply Zle_refl.
+exact Hstep.
 Qed.
 
 Theorem inbetween_step_Mi_Mi_even :
   forall x k,
-  inbetween (start + Z2R k * step) (start + Z2R (k + 1) * step) x loc_Eq ->
+  inbetween (start + Z2R k * step) (start + Z2R (k + 1) * step) x loc_Exact ->
   (2 * k = nb_steps)%Z ->
-  inbetween start (start + Z2R nb_steps * step) x loc_Mi.
+  inbetween start (start + Z2R nb_steps * step) x (loc_Inexact Eq).
 Proof.
 intros x k Hx Hk.
-constructor.
-inversion_clear Hx.
-rewrite <- Rplus_assoc.
-unfold Rdiv.
-rewrite Rmult_plus_distr_r.
-fold ((start + start)/2)%R.
-rewrite double_div2.
-rewrite H.
-apply f_equal.
-rewrite <- Hk, mult_Z2R.
+apply inbetween_step_not_Eq with (1 := Hx).
+omega.
+apply Rcompare_Eq.
+inversion_clear Hx as [Hx'|].
+rewrite Hx', <- Hk, mult_Z2R.
 simpl (Z2R 2).
-replace (2 * Z2R k * step * / 2)%R with (Z2R k * step * (2 * /2))%R by ring.
-rewrite Rinv_r, Rmult_1_r.
-apply refl_equal.
-now apply (Z2R_neq 2 0).
-Qed.
-
-Theorem inbetween_step_Mi_Mi_odd :
-  forall x k,
-  inbetween (start + Z2R k * step) (start + Z2R (k + 1) * step) x loc_Mi ->
-  (2 * k + 1 = nb_steps)%Z ->
-  inbetween start (start + Z2R nb_steps * step) x loc_Mi.
-Proof.
-intros x k Hx Hk.
-constructor.
-inversion_clear Hx.
-rewrite H.
-rewrite middle_odd with (1 := Hk).
-rewrite <- Rplus_assoc.
-unfold Rdiv.
-rewrite Rmult_plus_distr_r.
-fold ((start + start)/2)%R.
-now rewrite double_div2.
+field.
 Qed.
 
 Definition new_location_even k l :=
   if Zeq_bool k 0 then
-    match l with loc_Eq => loc_Eq | _ => loc_Lo end
+    match l with loc_Exact => l | _ => loc_Inexact Lt end
   else
+    loc_Inexact
     match Zcompare (2 * k) nb_steps with
-    | Lt => loc_Lo
-    | Eq => match l with loc_Eq => loc_Mi | _ => loc_Hi end
-    | Gt => loc_Hi
+    | Lt => Lt
+    | Eq => match l with loc_Exact => Eq | _ => Gt end
+    | Gt => Gt
     end.
 
 Theorem new_location_even_correct :
@@ -607,29 +373,25 @@ destruct (Zeq_bool_spec k 0) as [Hk0|Hk0].
 (* k = 0 *)
 rewrite Hk0 in Hx.
 rewrite Rmult_0_l, Rplus_0_r, Rmult_1_l in Hx.
-set (l' := match l with loc_Eq => loc_Eq | _ => loc_Lo end).
-assert ((l = loc_Eq /\ l' = loc_Eq) \/ (l <> loc_Eq /\ l' = loc_Lo)).
+set (l' := match l with loc_Exact => l | _ => loc_Inexact Lt end).
+assert ((l = loc_Exact /\ l' = loc_Exact) \/ (l <> loc_Exact /\ l' = loc_Inexact Lt)).
 unfold l' ; case l ; try (now left) ; right ; now split.
 destruct H as [(H1,H2)|(H1,H2)] ; rewrite H2.
 constructor.
 rewrite H1 in Hx.
 now inversion_clear Hx.
-now apply inbetween_step_Lo_Eq with (2 := H1).
+now apply inbetween_step_Lo_not_Eq with (2 := H1).
 (* k <> 0 *)
 destruct (Zcompare_spec (2 * k) nb_steps) as [Hk1|Hk1|Hk1].
 (* . 2 * k < nb_steps *)
 apply inbetween_step_Lo with (1 := Hx).
-case (Z_le_lt_eq_dec _ _ (proj1 Hk)).
-easy.
-intros H.
-rewrite <- H in Hk0.
-now elim Hk0.
+omega.
 destruct (Zeven_ex nb_steps).
 rewrite He in H.
 omega.
 (* . 2 * k = nb_steps *)
-set (l' := match l with loc_Eq => loc_Mi | _ => loc_Hi end).
-assert ((l = loc_Eq /\ l' = loc_Mi) \/ (l <> loc_Eq /\ l' = loc_Hi)).
+set (l' := match l with loc_Exact => Eq | _ => Gt end).
+assert ((l = loc_Exact /\ l' = Eq) \/ (l <> loc_Exact /\ l' = Gt)).
 unfold l' ; case l ; try (now left) ; right ; now split.
 destruct H as [(H1,H2)|(H1,H2)] ; rewrite H2.
 rewrite H1 in Hx.
@@ -643,12 +405,13 @@ Qed.
 
 Definition new_location_odd k l :=
   if Zeq_bool k 0 then
-    match l with loc_Eq => loc_Eq | _ => loc_Lo end
+    match l with loc_Exact => l | _ => loc_Inexact Lt end
   else
+    loc_Inexact
     match Zcompare (2 * k + 1) nb_steps with
-    | Lt => loc_Lo
-    | Eq => match l with loc_Mi => loc_Mi | loc_Hi => loc_Hi | _ => loc_Lo end
-    | Gt => loc_Hi
+    | Lt => Lt
+    | Eq => match l with loc_Inexact l => l | loc_Exact => Lt end
+    | Gt => Gt
     end.
 
 Theorem new_location_odd_correct :
@@ -663,31 +426,23 @@ destruct (Zeq_bool_spec k 0) as [Hk0|Hk0].
 (* k = 0 *)
 rewrite Hk0 in Hx.
 rewrite Rmult_0_l, Rplus_0_r, Rmult_1_l in Hx.
-set (l' := match l with loc_Eq => loc_Eq | _ => loc_Lo end).
-assert ((l = loc_Eq /\ l' = loc_Eq) \/ (l <> loc_Eq /\ l' = loc_Lo)).
+set (l' := match l with loc_Exact => l | _ => loc_Inexact Lt end).
+assert ((l = loc_Exact /\ l' = loc_Exact) \/ (l <> loc_Exact /\ l' = loc_Inexact Lt)).
 unfold l' ; case l ; try (now left) ; right ; now split.
 destruct H as [(H1,H2)|(H1,H2)] ; rewrite H2.
 constructor.
 rewrite H1 in Hx.
 now inversion_clear Hx.
-now apply inbetween_step_Lo_Eq with (2 := H1).
+now apply inbetween_step_Lo_not_Eq with (2 := H1).
 (* k <> 0 *)
 destruct (Zcompare_spec (2 * k + 1) nb_steps) as [Hk1|Hk1|Hk1].
 (* . 2 * k + 1 < nb_steps *)
 apply inbetween_step_Lo with (1 := Hx) (3 := Hk1).
-case (Z_le_lt_eq_dec _ _ (proj1 Hk)).
-easy.
-intros H.
-rewrite <- H in Hk0.
-now elim Hk0.
+omega.
 (* . 2 * k + 1 = nb_steps *)
 destruct l.
-apply inbetween_step_Lo_Mi_odd with (1 := Hx) (3 := Hk1).
-now left.
-apply inbetween_step_Lo_Mi_odd with (1 := Hx) (3 := Hk1).
-now right.
-apply inbetween_step_Mi_Mi_odd with (1 := Hx) (2 := Hk1).
-apply inbetween_step_Hi_Mi_odd with (1 := Hx) (2 := Hk1).
+apply inbetween_step_Lo_Mi_Eq_odd with (1 := Hx) (2 := Hk1).
+apply inbetween_step_any_Mi_odd with (1 := Hx) (2 := Hk1).
 (* . 2 * k + 1 > nb_steps *)
 apply inbetween_step_Hi with (1 := Hx).
 destruct (Zeven_ex nb_steps).
@@ -730,100 +485,71 @@ Hypothesis Hd : Rnd_DN_pt F x d.
 Hypothesis Hu : Rnd_UP_pt F x u.
 
 Theorem Rnd_N_pt_bracket_not_Hi :
-  forall l, l <> loc_Hi ->
+  forall l, l <> loc_Inexact Gt ->
   inbetween d u x l ->
   Rnd_N_pt F x d.
 Proof.
 intros l Hl Hx.
-split.
-apply Hd.
-intros g Hg.
-rewrite Rabs_left1. 2: apply Rle_minus ; apply Hd.
-rewrite Ropp_minus_distr.
-destruct (Rnd_DN_UP_pt_split  _ _ _ _ Hd Hu g Hg) as [H|H].
-rewrite Rabs_left1.
-rewrite Ropp_minus_distr.
-apply Rplus_le_compat_l.
-now apply Ropp_le_contravar.
-apply Rle_minus.
-apply Rle_trans with (1 := H).
-apply Hd.
-rewrite Rabs_pos_eq.
-apply Rplus_le_reg_r with (x + d)%R.
-ring_simplify.
-apply Rle_trans with (d + u)%R.
-apply Rmult_le_reg_l with (/2)%R.
-apply Rinv_0_lt_compat.
-now apply (Z2R_lt 0 2).
-rewrite <- Rmult_assoc, Rinv_l, Rmult_1_l.
-rewrite Rmult_comm.
-refine (proj2 (inbetween_not_Hi _ _ _ _ _ Hx Hl)).
+apply Rnd_DN_pt_N with (1 := Hd) (2 := Hu).
+inversion Hx as [Hx'|l' Hx' Hl'].
+rewrite Hx'.
+unfold Rminus.
+rewrite Rplus_opp_r.
+apply Rle_0_minus.
 apply Rle_trans with x.
 apply Hd.
 apply Hu.
-now apply (Z2R_neq 2 0).
-now apply Rplus_le_compat_l.
-apply Rle_0_minus.
-apply Rle_trans with (2 := H).
-apply Hu.
+apply Rcompare_not_Gt_inv.
+rewrite Rcompare_middle.
+rewrite Hl'.
+contradict Hl.
+now rewrite <- H, Hl.
 Qed.
 
 Theorem Rnd_N_pt_bracket_Mi_Hi :
-  forall l, l = loc_Mi \/ l = loc_Hi ->
+  forall l, l = loc_Inexact Eq \/ l = loc_Inexact Gt ->
   inbetween d u x l ->
   Rnd_N_pt F x u.
 Proof.
 intros l Hl Hx.
-split.
-apply Hu.
-intros g Hg.
-rewrite Rabs_pos_eq. 2: now apply Rle_0_minus ; apply Hu.
-destruct (Rnd_DN_UP_pt_split  _ _ _ _ Hd Hu g Hg) as [H|H].
-rewrite Rabs_left1.
-rewrite Ropp_minus_distr.
-apply Rplus_le_reg_r with (x + g)%R.
-ring_simplify.
-apply Rle_trans with (u + d)%R.
-now apply Rplus_le_compat_l.
-rewrite Rplus_comm.
-apply Rmult_le_reg_l with (/2)%R.
-apply Rinv_0_lt_compat.
-now apply (Z2R_lt 0 2).
-rewrite <- Rmult_assoc, Rinv_l, Rmult_1_l.
-rewrite Rmult_comm.
-refine (proj1 (inbetween_Mi_Hi _ _ _ _ _ Hx Hl)).
-apply Rle_trans with x.
-apply Hd.
-apply Hu.
-now apply (Z2R_neq 2 0).
-apply Rle_minus.
-apply Rle_trans with (1 := H).
-apply Hd.
-rewrite Rabs_pos_eq.
-now apply Rplus_le_compat_r.
-apply Rle_0_minus.
-apply Rle_trans with (2 := H).
-apply Hu.
+apply Rnd_UP_pt_N with (1 := Hd) (2 := Hu).
+inversion Hx as [Hx' Hl'|l' Hx' Hl' Hl''].
+now destruct Hl as [Hl|Hl] ; rewrite Hl in Hl'.
+apply Rcompare_not_Lt_inv.
+rewrite Rcompare_middle.
+rewrite Hl'.
+intros H.
+rewrite H in Hl''.
+rewrite <- Hl'' in Hl.
+now destruct Hl.
 Qed.
 
 Theorem Rnd_not_N_pt_bracket_Hi :
-  inbetween d u x loc_Hi ->
+  inbetween d u x (loc_Inexact Gt) ->
   ~ Rnd_N_pt F x d.
 Proof.
 intros Hx (_, Hn).
 specialize (Hn u (proj1 Hu)).
 apply Rle_not_lt with (1 := Hn).
-now apply inbetween_distance_Hi.
+apply Rcompare_Gt_inv.
+apply inbetween_distance_inexact_abs.
+refine (let H := _ in Rlt_trans _ x _ (proj1 H) (proj2 H)).
+now apply inbetween_bounds_not_Eq with (1 := Hx).
+exact Hx.
 Qed.
 
 Theorem Rnd_not_N_pt_bracket_Lo :
-  inbetween d u x loc_Lo ->
+  inbetween d u x (loc_Inexact Lt) ->
   ~ Rnd_N_pt F x u.
 Proof.
 intros Hx (_, Hn).
 specialize (Hn d (proj1 Hd)).
 apply Rle_not_lt with (1 := Hn).
-now apply inbetween_distance_Lo.
+apply Rcompare_Lt_inv.
+apply inbetween_distance_inexact_abs.
+refine (let H := _ in Rlt_trans _ x _ (proj1 H) (proj2 H)).
+now apply inbetween_bounds_not_Eq with (1 := Hx).
+exact Hx.
 Qed.
 
 End Fcalc_bracket_N.
@@ -844,17 +570,11 @@ Theorem inbetween_mult_compat :
   inbetween x d u l ->
   inbetween (x * s) (d * s) (u * s) l.
 Proof.
-intros x d u l s Hs Hl.
-destruct Hl as [Hl|Hl1 Hl2|Hl|Hl1 Hl2] ; constructor.
-now apply (f_equal (fun v => (v * s)%R)).
-now apply Rmult_lt_compat_r.
+intros x d u l s Hs [Hx|l' Hx Hl] ; constructor.
+now rewrite Hx.
+now split ; apply Rmult_lt_compat_r.
 rewrite inbetween_mult_aux.
-now apply Rmult_lt_compat_r.
-rewrite Hl.
-field.
-rewrite inbetween_mult_aux.
-now apply Rmult_lt_compat_r.
-now apply Rmult_lt_compat_r.
+now rewrite Rcompare_mult_r.
 Qed.
 
 Theorem inbetween_mult_reg :
@@ -863,19 +583,12 @@ Theorem inbetween_mult_reg :
   inbetween (x * s) (d * s) (u * s) l ->
   inbetween x d u l.
 Proof.
-intros x d u l s Hs Hl.
-destruct Hl as [Hl|Hl1 Hl2|Hl|Hl1 Hl2] ; constructor.
-apply Rmult_eq_reg_r with (1 := Hl).
+intros x d u l s Hs [Hx|l' Hx Hl] ; constructor.
+apply Rmult_eq_reg_r with (1 := Hx).
 now apply Rgt_not_eq.
-now apply Rmult_lt_reg_r with (1 := Hs).
-apply Rmult_lt_reg_r with (1 := Hs).
-now rewrite <- inbetween_mult_aux.
-apply Rmult_eq_reg_r with s.
-now rewrite <- inbetween_mult_aux.
-now apply Rgt_not_eq.
-apply Rmult_lt_reg_r with (1 := Hs).
-now rewrite <- inbetween_mult_aux.
-now apply Rmult_lt_reg_r with (1 := Hs).
+now split ; apply Rmult_lt_reg_r with s.
+rewrite <- Rcompare_mult_r with (1 := Hs).
+now rewrite inbetween_mult_aux in Hl.
 Qed.
 
 End Fcalc_bracket_scale.
@@ -946,26 +659,6 @@ apply bpow_gt_0.
 now rewrite scaled_mantissa_bpow.
 Qed.
 
-Theorem inbetween_float_rounding_pos :
-  forall rnd choice,
-  ( forall x m l, (0 < x)%R -> inbetween_int m x l -> Zrnd rnd x = choice m l ) ->
-  forall x m l, (0 < x)%R ->
-  let e := canonic_exponent beta fexp x in
-  inbetween_float m e x l ->
-  rounding beta fexp rnd x = F2R (Float beta (choice m l) e).
-Proof.
-intros rnd choice Hc x m l Hx e Hl.
-unfold rounding, F2R. simpl.
-apply (f_equal (fun m => (Z2R m * bpow e)%R)).
-apply Hc.
-apply Rmult_lt_0_compat.
-exact Hx.
-apply bpow_gt_0.
-apply inbetween_mult_reg with (bpow e).
-apply bpow_gt_0.
-now rewrite scaled_mantissa_bpow.
-Qed.
-
 Theorem inbetween_float_DN :
   forall x m l,
   let e := canonic_exponent beta fexp x in
@@ -975,7 +668,7 @@ Proof.
 apply inbetween_float_rounding with (choice := fun m l => m).
 intros x m l Hl.
 apply Zfloor_imp.
-apply inbetween_bounds_strict with (2 := Hl).
+apply inbetween_bounds with (2 := Hl).
 apply Z2R_lt.
 apply Zlt_succ.
 Qed.
@@ -984,7 +677,7 @@ Definition cond_incr (b : bool) m := if b then (m + 1)%Z else m.
 
 Definition round_UP l :=
   match l with
-  | loc_Eq => false
+  | loc_Exact => false
   | _ => true
   end.
 
@@ -996,149 +689,60 @@ Theorem inbetween_float_UP :
 Proof.
 apply inbetween_float_rounding with (choice := fun m l => cond_incr (round_UP l) m).
 intros x m l Hl.
-assert (Hl': l = loc_Eq \/ (l <> loc_Eq /\ round_UP l = true)).
+assert (Hl': l = loc_Exact \/ (l <> loc_Exact /\ round_UP l = true)).
 case l ; try (now left) ; now right ; split.
 destruct Hl' as [Hl'|(Hl1, Hl2)].
-(* loc_Eq *)
+(* Exact *)
 rewrite Hl'.
 destruct Hl ; try easy.
 rewrite H.
 apply Zceil_Z2R.
-(* not loc_Eq *)
+(* not Exact *)
 rewrite Hl2.
 simpl.
 apply Zceil_imp.
 ring_simplify (m + 1 - 1)%Z.
 refine (let H := _ in conj (proj1 H) (Rlt_le _ _ (proj2 H))).
-apply inbetween_bounds_strict_not_Eq with (3 := Hl1) (2 := Hl).
-apply Z2R_lt.
-apply Zlt_succ.
+apply inbetween_bounds_not_Eq with (2 := Hl1) (1 := Hl).
 Qed.
 
 Definition round_NE (p : bool) l :=
   match l with
-  | loc_Eq => false
-  | loc_Lo => false
-  | loc_Mi => if p then false else true
-  | loc_Hi => true
+  | loc_Exact => false
+  | loc_Inexact Lt => false
+  | loc_Inexact Eq => if p then false else true
+  | loc_Inexact Gt => true
   end.
 
-Hypothesis strong_fexp : NE_ex_prop beta fexp.
-
 Theorem inbetween_float_NE :
-  forall x m l, (0 < x)%R ->
+  forall x m l,
   let e := canonic_exponent beta fexp x in
   inbetween_float m e x l ->
-  Rnd_NE_pt beta fexp x (F2R (Float beta (cond_incr (round_NE (Zeven m) l) m) e)).
+  rounding beta fexp ZrndNE x = F2R (Float beta (cond_incr (round_NE (Zeven m) l) m) e).
 Proof.
-intros x m l Hx e Hl.
-assert (Hd := inbetween_float_DN _ _ _ Hl).
-unfold round_NE.
-generalize (inbetween_float_UP _ _ _ Hl).
-fold e in Hd |- *.
-assert (Hd': Rnd_DN_pt format x (F2R (Float beta m e))).
-rewrite <- Hd.
-now apply generic_DN_pt.
-assert (Hu': Rnd_UP_pt format x (rounding beta fexp ZrndUP x)).
-now apply generic_UP_pt.
-destruct l ; simpl ; intros Hu.
-(* loc_Eq *)
-inversion_clear Hl.
-rewrite H.
-apply Rnd_NG_pt_refl.
-rewrite <- Hd.
-now apply generic_format_rounding.
-(* loc_Lo *)
-split.
-rewrite Hu in Hu'.
-now apply (Rnd_N_pt_bracket_not_Hi _ _ _ _ Hd' Hu' loc_Lo).
-right.
-intros g Hg.
-destruct (generic_N_pt_DN_or_UP _ _ prop_exp _ _ Hg) as [H|H].
-now rewrite <- Hd.
-rewrite H in Hg.
-elim (Rnd_not_N_pt_bracket_Lo _ _ _ _ Hd' Hl).
-now rewrite <- Hu.
-(* loc_Mi *)
-assert (Hm: (0 <= m)%Z).
-apply Zlt_succ_le.
-apply F2R_gt_0_reg with beta e.
-apply Rlt_le_trans with (1 := Hx).
-unfold Zsucc.
-rewrite <- Hu.
-apply (generic_UP_pt beta fexp prop_exp x).
-destruct (Z_le_lt_eq_dec _ _ Hm) as [Hm'|Hm'].
-(* - 0 < m *)
-assert (Hcd : canonic beta fexp (Float beta m e)).
-unfold canonic.
-apply sym_eq.
-rewrite <- Hd.
-apply canonic_exponent_DN ; try easy.
-rewrite Hd.
-now apply F2R_gt_0_compat.
-case_eq (Zeven m) ; intros Heo.
-split.
-apply (Rnd_N_pt_bracket_not_Hi _ _ _ _ Hd' Hu' loc_Mi).
-easy.
-now rewrite Hu.
-left.
-now eexists ; repeat split.
-split.
-rewrite Hu in Hu'.
-apply (Rnd_N_pt_bracket_Mi_Hi _ _ _ _ Hd' Hu' loc_Mi).
-now left.
-exact Hl.
-left.
-generalize (proj1 Hu').
-rewrite Hu.
-unfold generic_format.
-fold e.
-set (cu := Float beta (Ztrunc (scaled_mantissa beta fexp (F2R (Float beta (m + 1) e))))
-  (canonic_exponent beta fexp (F2R (Float beta (m + 1) e)))).
-intros Hu''.
-assert (Hcu : canonic beta fexp cu).
-unfold canonic.
-now rewrite <- Hu''.
-simpl.
-rewrite Hu''.
-eexists ; repeat split.
-exact Hcu.
-rewrite (DN_UP_parity_generic beta fexp prop_exp strong_fexp x (Float beta m e) cu) ; try easy.
-simpl.
-now rewrite Heo.
-apply (generic_format_discrete beta fexp x m).
-apply inbetween_bounds_strict_not_Eq with (2 := Hl).
-apply F2R_lt_compat.
-apply Zlt_succ.
-easy.
-now rewrite <- Hu''.
-(* - m = 0 *)
-case_eq (Zeven m) ; intros Heo.
-split.
-apply (Rnd_N_pt_bracket_not_Hi _ _ _ _ Hd' Hu' loc_Mi).
-easy.
-now rewrite Hu.
-left.
-rewrite <- Hm', F2R_0.
-exists (Float beta 0 (canonic_exponent beta fexp 0)).
-unfold canonic.
-rewrite F2R_0.
-repeat split.
-now rewrite <- Hm' in Heo.
-(* loc_Hi *)
-split.
-rewrite Hu in Hu'.
-apply (Rnd_N_pt_bracket_Mi_Hi _ _ _ _ Hd' Hu' loc_Hi).
-now right.
-exact Hl.
-right.
-intros g Hg.
-destruct (generic_N_pt_DN_or_UP _ _ prop_exp _ _ Hg) as [H|H].
-rewrite H in Hg.
-rewrite Hu in Hu'.
-elim (Rnd_not_N_pt_bracket_Hi _ _ _ _ Hu' Hl).
-now rewrite <- Hd.
-now rewrite H.
+apply inbetween_float_rounding with (choice := fun m l => cond_incr (round_NE (Zeven m) l) m).
+intros x m l Hl.
+inversion_clear Hl as [Hx|l' Hx Hl'].
+(* Exact *)
+rewrite Hx.
+now rewrite Zrnd_Z2R.
+(* not Exact *)
+unfold Zrnd, ZrndNE, ZrndN, Znearest.
+assert (Hm: Zfloor x = m).
+apply Zfloor_imp.
+exact (conj (Rlt_le _ _ (proj1 Hx)) (proj2 Hx)).
+rewrite Zceil_floor_neq.
+rewrite Hm.
+replace (Rcompare (x - Z2R m) (/2)) with l'.
+now case l'.
+rewrite <- Hl'.
+rewrite plus_Z2R.
+rewrite <- (Rcompare_plus_r (- Z2R m) x).
+apply f_equal.
+simpl (Z2R 1).
+field.
+rewrite Hm.
+now apply Rlt_not_eq.
 Qed.
 
 End Fcalc_bracket_generic.
